examples/mutsum/MutAll.v
@@ -2,25 +2,34 @@ Require Import CRIS Cancel.
 
 Require Import MutHeader MutMainHeader MutFA MutGA MutMainA.
 Require Import MutFI MutGI MutMainI.
-Require Import MutIAproof MutMainIAproof.
+Require Import MutFIAproof MutGIAproof MutMainIAproof.
+Require Import APCHeader APC APCI APCA APCC.
+Require Import APCIAproof APCACproof.
 
 Module MutAll.
   Import inv_instances.
   Local Instance Γ : HRA := ##[invΓ].
   Local Instance Σ : GRA := ##[invΣ; Γ].
 
-  Local Definition smod_src : SMod.t := MutMainA.Mod ☆ MutFA.Mod ☆ MutGA.Mod.
-  Local Definition stb : string → option fspec := spc_from smod_src.
+  Local Definition u : nat := 1.
+  Local Definition ginv : iProp Σ := wsim_ginv u ⊤.
+
+  Local Definition smod_src : SMod.t := MutMainA.Mod ☆ MutFA.Mod ☆ MutGA.Mod ☆ APCC.Mod.
+  Local Definition spc : string → option fspec := spc_from smod_src.
+
+  Local Definition smod_pure : SMod.t := MutFA.Mod ☆ MutGA.Mod.
+  Local Definition spc_pure : string → option fspec := spc_from smod_pure.
+
   Local Definition mod_cancel : HMod.t := SModCancel.to_hmod smod_src.
-  Local Definition mod_src : HMod.t := SMod.to_hmod emp stb smod_src.
-  Local Definition mod_tgt : HMod.t := MutMainI.t ★ MutFI.t ★ MutGI.t.
+  Local Definition mod_src : HMod.t := SMod.to_hmod ginv spc smod_src.
+  Local Definition mod_tgt : HMod.t := MutMainI.t ★ MutFI.t ★ MutGI.t ★ APCI.t.
 
   Local Definition main_fsp : fspec := MutMainA.main_spec.
   Local Definition init_cond : iProp Σ := MutFA.InitCond ∗ MutGA.InitCond.
 
   (* Apply cancellation to linked spec module *)
   Lemma cancel_src :
-    refines (mod_cancel, (init_cond ∗ main_fsp.(precond) 0 tt tt↑ tt↑)%I)
+    refines (mod_cancel, (init_cond ∗ main_fsp.(precond) tt tt↑ tt↑)%I)
             ((mod_src, init_cond) : HMod.modc).
   Proof.
     eapply cancellation; try by econs.
@@ -28,30 +37,55 @@ Module MutAll.
     des; eauto.
   Qed.
 
+  Ltac prove_spc :=
+    rewrite /APCA.Spc /MutFA.SpcF /MutGA.SpcG /spc /smod_src /spc_pure /spc_incl /spc_sub /find_body /pure_specbody /spc_from /smod_pure /option_map; try unseal CRIS; try prove_nodup;
+    ii; ss; rewrite ->!eq_rel_dec_correct in *; des_ifs; eexists; ss.
+
   (* Refinement between spec/impl of whole program (linked module) *)
   Lemma src_tgt : refines (mod_src, init_cond) (mod_tgt, emp%I).
   Proof.
     eapply ctxr_refines.
     (* rewrite -[(mod_tgt, _)]hmod_addc_empty_r. *)
     unfold mod_src, mod_tgt. rewrite !add_interp_comm.
-    rewrite -hmod_add_assoc.
+    do 2 rewrite -hmod_add_assoc.
+    etrans. { eapply ctxr_comm. }
     etrans.
-    { rewrite -hmod_addc_empty_l. eapply ctxr_cond_frameR. eapply ctxr_frameR.
-      replace (SMod.to_hmod emp stb MutMainA.Mod) with (MutMainA.t stb); cycle 1.
-      { unfold MutMainA.t. unseal CRIS. ss. }
-      replace (SMod.to_hmod emp stb MutFA.Mod) with (MutFA.t stb); cycle 1.
-      { unfold MutFA.t. unseal CRIS. ss. }
-      apply MutMainIA.correct.
+    { rewrite -hmod_addc_empty_l. eapply ctxr_cond_frameR.
+      replace (SMod.to_hmod ginv spc APCC.Mod) with (APCC.t 1 spc); cycle 1.
+      { unfold APCC.t. unseal CRIS. ss. }
+      eapply APCAC.wctxr.
+      { instantiate (1:=spc). prove_spc. }
+      { instantiate (1:=spc_pure). prove_spc. } 
+      { prove_spc. }
     }
-    rewrite hmod_add_assoc hmod_addc_empty_l.
+    etrans. { eapply ctxr_comm. }
+    rewrite !hmod_add_assoc. rewrite -(hmod_add_assoc (SMod.to_hmod ginv spc MutFA.Mod)).
+    etrans.
+    { eapply ctxr_compose_mix.
+      { replace (SMod.to_hmod ginv spc MutMainA.Mod) with (MutMainA.t 1 spc); cycle 1.
+        { unfold MutMainA.t. unseal CRIS. ss. }
+        eapply MutMainIA.wctxr; prove_spc.
+      }
+      { replace (SMod.to_hmod ginv spc MutFA.Mod) with (MutFA.t 1 spc); cycle 1.
+        { unfold MutFA.t. unseal CRIS. ss. }
+        replace (SMod.to_hmod ginv spc MutGA.Mod) with (MutGA.t 1 spc); cycle 1.
+        { unfold MutGA.t. unseal CRIS. ss. }
+        rewrite !hmod_add_assoc.
+        etrans.
+        { eapply ctxr_compose_mix.
+          { eapply MutFIA.wctxr; prove_spc. }
+          { eapply MutGIA.wctxr; prove_spc. }
+        }
+        rewrite hmod_addc_empty_l -hmod_add_assoc. refl.
+      }
+    }
+    rewrite hmod_addc_empty_l -!hmod_add_assoc.
     eapply ctxr_frameL.
-    replace (SMod.to_hmod emp stb MutGA.Mod) with (MutGA.t stb); cycle 1.
-    { unfold MutGA.t. unseal CRIS. ss. }
-    apply MutIA.correct.
+    eapply APCIA.wctxr.
   Qed.
 
   Lemma cancel_tgt :
-    refines (mod_cancel, (init_cond ∗ main_fsp.(precond) 0 tt tt↑ tt↑)%I)
+    refines (mod_cancel, (init_cond ∗ main_fsp.(precond) tt tt↑ tt↑)%I)
             (mod_tgt, emp%I).
   Proof.
     etrans.
