examples/mutsum/MutFA.v
@@ -5,7 +5,7 @@ Set Implicit Arguments.
 
 Module MutFA. Section MutFA.
   Import MutAUX.
-  Context {Σ: GRA}.
+  Context `{!invG α Σ Γ, !subG Γ Σ, !sinvG Σ Γ α β τ}.
   Notation iProp := (iProp Σ).
 
   Definition scopes := ["MutF"].
@@ -36,5 +36,5 @@ Module MutFA. Section MutFA.
 
   Definition InitCond : iProp := emp%I.
 
-  Definition t Spc := Seal.sealing CRIS (SMod.to_hmod emp Spc Mod).
+  Definition t u Spc := Seal.sealing CRIS (SMod.to_hmod (wsim_ginv u ⊤) Spc Mod).
 End MutFA. End MutFA.
