examples/mutsum/MutGIAproof.v
@@ -1,0 +1,103 @@
+Require Import CRIS.
+
+Require Import NormITree.
+Require Import MutHeader MutGI MutGA MutFA.
+Require Import APCHeader APC APCA.
+
+Set Implicit Arguments.
+
+Module MutGIA. Section MutGIA.
+  Import MutAUX.
+  Context `{!invG α Σ Γ, !subG Γ Σ, !sinvG Σ Γ α β τ}.
+
+  Context (u_s u_apc: univ_id).
+  Context (Spc: string -> option fspec).
+  Context (SpcPure: string -> option fspec).
+
+  Context (APCInSpc : spc_incl (APCA.Spc) Spc).
+  Context (FInPure : spc_incl (MutFA.SpcF) SpcPure).
+  Context (PureInSpc : spc_sub SpcPure Spc).
+
+  Definition Ist: nat -> alist key Any.t -> alist key Any.t -> iProp Σ :=
+    λ _ _ _, (True)%I.
+
+  Local Definition MutGAMod := (MutGA.t u_s Spc ★ APCA.t u_apc SpcPure Spc).
+  Local Definition MutGIMod := (MutGI.t ★ APCA.t u_apc SpcPure Spc).
+  Local Definition IstFull := (IstProd (IstSB (MutGA.t u_s Spc).(HMod.scopes) Ist) IstEq).
+  
+  (*************)
+
+  Lemma simF_mutg:
+    HSim.sim_fun open MutGAMod MutGIMod IstFull MutName.mutg.
+  Proof.
+    winit_simF u_s 0.
+
+    wsteps_l. iDestruct "ASM" as "((%Y & %B) & %Q)". subst; hss.
+    wsteps_r. unfold assume. wforce_r. wsteps_r.
+    
+    destruct q; s.
+    { (* f(0) *)
+      wsteps_r. wforce_l. wsteps_l.
+      wforces_l. iSplitR; et. wsteps_l. 
+      winline_l. wsteps_l. iDestruct "ASM" as "[-> <-]"; hss. wsteps_l.
+      rewrite /APC. wforce_l q. wsteps_l. rewrite unfold_APC.
+      wforce_l true. wsteps_l. wforces_l. iSplitR; eauto.
+      wsteps_l. wforces_l. iSplitR; eauto.
+      wstep. iSplitR "IST"; iFrame; auto.
+    }
+
+    replace (S q - 1)%Z with (Z.of_nat q) by nia.
+    wsteps_l. wforce_l vo. wsteps_l. wforces_l. iSplitR; eauto.
+    winline_l. wsteps_l. iDestruct "ASM" as "[-> <-]"; hss. wsteps_l.
+    rewrite /APC. wforce_l 1. wsteps_l. rewrite unfold_APC.
+    wforce_l false. wsteps_l. wforce_l 0. wsteps_l.
+    assert (LT: (0 < 1)%ord).
+    { eapply OrdArith.lt_from_nat. nia. }
+    wforce_l LT. wsteps_l. wforce_l MutName.mutf. wsteps_l. wforce_l q. wsteps_l.
+    assert (is_Some (SpcPure MutName.mutf) ∧ (q < vo)%ord).
+    { split. 
+      { rewrite /is_Some. unfold MutFA.SpcF in FInPure.
+        revert FInPure. unseal CRIS. i. unfold spc_incl in FInPure.
+        destruct FInPure. rewrite /spc_sub /to_spc in H0.
+        hexploit (H0 MutName.mutf MutFA.f_spec); [refl|]. i. eauto.
+      }
+      { eapply Ord.lt_le_lt; eauto. eapply OrdArith.lt_from_nat. nia. }
+    }
+    unfold guarantee. wforce_l H. wsteps_l. wforce_l. iSplitR.
+    { iPureIntro. eapply PureInSpc. eapply FInPure. rewrite /MutFA.SpcF. unseal CRIS. ss. }
+    wsteps_l. wforce_l q. wsteps_l. wforces_l. iSplitR; eauto.
+    { iPureIntro. esplits; eauto.
+      { nia. } { refl. }
+    }
+    wcall "IST". wsteps_l. iDestruct "ASM" as "->"; hss. wsteps_r. hss. wsteps_r.
+    rewrite unfold_APC. wforce_l true. wsteps_l. wforces_l. iSplitR; first done.
+    wsteps_l. wforces_l; iSplitR; eauto; iClear "ASM".
+    wstep. iFrame. iPureIntro. do 2 f_equal. nia.
+    Unshelve. all: ss.
+    { eapply mut_max_intrange; eauto. }
+    { exact (0↑). }
+  Qed.
+
+  Theorem sim:
+    HSim.t open MutGAMod MutGIMod MutGA.InitCond IstFull.
+  Proof.
+    init_sim.
+    - iIntros "C". iExists [], [], [], []. do 2 iSplit; eauto. iFrame. iPureIntro.
+      rewrite /MutGA.scopes /state_scopes /incl //.
+    - eapply simF_mutg.
+  Qed.
+End MutGIA.
+
+Section wctxr.
+  Context `{!invG α Σ Γ, !subG Γ Σ, !sinvG Σ Γ α β τ}.
+
+  Theorem wctxr (u_s u_apc: univ_id) (Spc SpcPure: string → option fspec) 
+    (APCInSpc : spc_incl (APCA.Spc) Spc)
+    (FInPure : spc_incl (MutFA.SpcF) SpcPure)
+    (PureInSpc : spc_sub SpcPure Spc)
+  :
+    ctx_refines
+      (MutGA.t u_s Spc ★ APCA.t u_apc SpcPure Spc, MutGA.InitCond)
+      (MutGI.t ★ APCA.t u_apc SpcPure Spc, emp%I).
+  Proof. eapply main_adequacy, sim; eauto. Qed.
+End wctxr. End MutGIA.
